UTP/ITree_Circus.thy
@@ -312,6 +312,9 @@ definition promote :: "('e, 's\<^sub>1) htree \<Rightarrow> ('s\<^sub>1 \<Longri
 syntax "_promote" :: "logic \<Rightarrow> svid \<Rightarrow> logic" (infix "\<Up>\<Up>" 60)
 translations "_promote P a" == "CONST promote P a"
 
+definition action_system :: "('s \<Rightarrow> 'e \<Zpfun> 's) \<Rightarrow> ('e, 's) htree"
+  where "action_system P = loop (\<lambda> s. Vis (map_pfun (\<lambda> s'. Ret s') (P s)))"
+
 named_theorems prog_defs
 
 end
